Good progress on scopability proofs

Reachability.v
@@ -17,73 +17,8 @@ Module Reachability.
   |rch_trans : forall l0 l1 l2 C ω σ, (reachability σ l0 l1) -> (getObj σ l1 = Some (C, ω)) -> (exists f, (getVal ω f = Some l2)) -> (l2 < dom σ) -> (reachability σ l0 l2).
   Notation "σ ⊨ l1 ⇝ l2" := (reachability σ l1 l2) (at level 80, l1 at level 80, l2 at level 80).
 
-
-  Definition reachable_one_step σ l0 l1 :=
-    exists C ω, (getObj σ l0 = Some (C, ω)) /\ (exists f, (getVal ω f = Some l1)) /\ (l1 < dom σ).
-
-  Lemma reachable_one_step_reachability :
-    forall σ l0 l1, reachable_one_step σ l0 l1 -> σ ⊨ l0 ⇝ l1.
-  Proof.
-    unfold reachable_one_step; steps.
-    eauto using rch_trans, rch_heap, getObj_dom.
-  Qed.
-
-  (* Path in σ to e (p is in reverse order) *)
-  Fixpoint reachable_path σ e p :=
-    match p with
-    | l::nil => (* p = [l] *)
-      l = e /\ e < dom σ
-    | l::p' => (* p = p'++[l] *)
-      (reachable_one_step σ l e) /\ (reachable_path σ l p')
-    | _ => False
-    end.
-
-  Lemma reachable_path_reachability:
-    forall σ s e,
-      (exists p, reachable_path σ e (p++[s])) <-> σ ⊨ s ⇝ e.
-  Proof.
-    split.
-    + intros [p Hp].
-      generalize dependent e.
-      induction p; repeat light; eauto using rch_heap.
-      destruct_match; [destruct p; steps | repeat light].
-      unfold reachable_one_step in H. move: H => [C [ω H]]. light.
-      eapply rch_trans; eauto.
-    + induction 1; steps.
-      ++ exists []; simpl; eauto.
-      ++ exists (l1::p); simpl. destruct (p++[l0]) eqn:P ; [destruct p ; steps | idtac].
-         rewrite P; rewrite <- P.
-         split; eauto.
-         unfold reachable_one_step.
-         eexists; eexists; eauto.
-  Qed.
-
-  Lemma reachable_path_is_reachable:
-    forall σ e p l,
-      reachable_path σ e p ->
-      List.In l p ->
-      σ ⊨ l ⇝ e.
-  Proof.
-    intros σ e p.
-    generalize dependent e.
-    induction p ; try solve [repeat light].
-    intros. simpl in H0. destruct H0 as [H0 | H0].
-    + subst; simpl in H.
-      destruct p eqn:P ; repeat light; eauto using rch_heap, reachable_one_step_reachability.
-    + simpl in H.
-      destruct p eqn:P; eauto using in_nil.
-      rewrite <- P in *.
-      destruct_and.
-      unfold reachable_one_step in *.
-      Opaque reachable_path.
-      move: H => [C [ ω [ Hobj [[f H] Hdom]] ] ] .
-      eapply IHp in H1; eauto using rch_trans.
-  Qed.
-
-
   Definition reachability_set σ (L: LocSet) l := exists l', (l' ∈ L) /\ (σ ⊨ l' ⇝ l).
   Notation "σ ⊫ L ⇝ l" := (reachability_set σ L l) (at level 80, l at level 99, L at level 99).
-
 
   Definition reachable_cold (σ: Store) (l: Loc) := (l < dom σ).
   Notation "σ ⊨ l : 'cold'" := (reachable_cold σ l) (at level 80, l at level 80).
@@ -121,11 +56,209 @@ Module Reachability.
     induction H; steps.
   Qed.
 
-
-
-
-
   (* Notions of path into the heap *)
+
+
+
+  Definition reachable_one_step σ l0 l1 :=
+    exists C ω, (getObj σ l0 = Some (C, ω)) /\ (exists f, (getVal ω f = Some l1)) /\ (l1 < dom σ).
+
+  Lemma reachable_one_step_reachability :
+    forall σ l0 l1, reachable_one_step σ l0 l1 -> σ ⊨ l0 ⇝ l1.
+  Proof.
+    unfold reachable_one_step; steps.
+    eauto using rch_trans, rch_heap, getObj_dom.
+  Qed.
+
+  (* Path in σ (p is in reverse order) *)
+  Fixpoint reachable_path σ p {struct p}:=
+    match p with
+    | [] => True
+    | l1::nil => l1 < dom σ
+    | l2::((l1::_) as p') => reachable_one_step σ l1 l2 /\ reachable_path σ p'
+    end.
+
+  Ltac destructs :=
+    repeat subst ||
+    match goal with
+    | H : _ \/ _ |- _ => let fresh1 := fresh H in
+                      let fresh2 := fresh H in destruct H as [fresh1 | fresh2]
+    | H : _ /\ _ |- _ => let fresh1 := fresh H in
+                      let fresh2 := fresh H in destruct H as [fresh1 fresh2]
+    | H : exists a, _  |- _ => let fresh a := fresh a in destruct H as [a H]
+    end.
+
+
+  Lemma reachable_path_reachability:
+    forall σ s e,
+      ((s = e /\ s < dom σ) \/ exists p, reachable_path σ (e :: (p++[s]))) <-> σ ⊨ s ⇝ e.
+  Proof.
+    split.
+    + intros [[H1 H2] | [p Hp]]; subst; eauto using rch_heap.
+      generalize dependent e.
+      generalize dependent s.
+      induction p; repeat light; eauto using reachable_one_step_reachability.
+      specialize (IHp s a).
+         unfold reachable_one_step in H. destructs.
+         eapply rch_trans; eauto.
+    + induction 1 ; [steps | destructs].
+      ++ right. exists []. simpl; unfold reachable_one_step; steps.
+         repeat eexists; eauto.
+      ++ right. exists (l1::p); simpl.
+         split; eauto.
+         eexists; eexists; eauto.
+  Qed.
+
+  Lemma reachable_path_is_reachable:
+    forall σ e p l,
+      reachable_path σ (e::p) ->
+      List.In l p ->
+      σ ⊨ l ⇝ e.
+  Proof.
+    intros σ e p.
+    generalize dependent e.
+    induction p ; try solve [repeat light].
+    intros. simpl in H0. destruct H0 as [H0 | H0].
+    + subst; simpl in H.
+      destruct p eqn:P ; repeat light; eauto using rch_heap, reachable_one_step_reachability.
+    + specialize (IHp a l).
+      destruct p eqn:P; try solve [exfalso; eauto using in_nil].
+      rewrite <- P in *. simpl in H.
+      destruct_and.
+      unfold reachable_one_step in H.
+      destructs.
+      eapply rch_trans; eauto.
+      eapply IHp; simpl; eauto.
+  Qed.
+
+  Lemma reachable_path_last:
+    forall σ s1 s2 p,
+      reachable_path σ (p++[s2;s1]) ->
+      reachable_path σ (p++[s2]).
+  Proof.
+    intros.
+    induction p; simpl in *.
+    + unfold reachable_one_step in * ; steps.
+    + destruct_match; [ apply_anywhere app_eq_nil; steps | ].
+      destruct_match; [ apply_anywhere app_eq_nil; steps | ].
+      assert ( n = n0) by (destruct p; steps); steps.
+  Qed.
+
+
+  Lemma reachable_path_app:
+    forall σ s1 s2 p1 p2,
+      reachable_path σ (p2++s2::p1++[s1]) ->
+      reachable_path σ (s2::p1++[s1]) /\ reachable_path σ (p2++[s2]).
+  Proof.
+    split; intros.
+    + generalize dependent s1.
+      generalize dependent s2.
+      generalize dependent p1.
+      induction p2; simpl.
+      ++ destruct p1; steps.
+      ++ intros. repeat ( destruct_match; [apply_anywhere app_eq_nil; steps |]).
+         rewrite <- matched in *.
+         rewrite <- matched0 in *.
+         destructs.
+         apply IHp2 in H1. simpl in H1.
+         steps.
+    + assert (forall l p s, reachable_path σ (p++s::l) -> reachable_path σ (p++[s])); eauto.
+      induction l; steps.
+      specialize (IHl (p++[s]) a).
+      eapply reachable_path_last.
+      repeat rewrite <- app_assoc in *.
+      simpl in *; eauto.
+  Qed.
+
+  Definition contains_edge p (l1 l2 :Loc) :=
+    exists p1 p2, p = p2 ++ l2::l1::p1.
+
+  Lemma contains_edge_dec :
+    forall p l1 l2, contains_edge p l1 l2 \/ not (contains_edge p l1 l2).
+  Proof.
+    unfold contains_edge. intros.
+    induction p; steps.
+    + right. steps. symmetry in H. apply app_eq_nil in H. steps.
+    + left. exists p1, (a::p2); steps.
+    + pose proof (PeanoNat.Nat.eq_dec a l2) as [Ha | Ha].
+      ++ (* a = l2 *)
+        subst.
+        destruct p; steps.
+        +++ right; steps. symmetry in H0. apply app_eq_unit in H0; steps.
+        +++ pose proof (PeanoNat.Nat.eq_dec l l1) as [Hl | Hl].
+            ++++ left; steps.
+                 exists p, []; steps.
+            ++++ right; steps. destruct p2; steps; eauto.
+      ++ right; steps.
+         destruct p2; steps; eauto.
+  Qed.
+
+
+  Lemma reachable_path_split_on_edge:
+    forall σ s p l1 l2,
+      reachable_path σ (p++[s]) ->
+      contains_edge p l1 l2 ->
+      σ ⊨ s ⇝ l1.
+  Proof.
+    unfold contains_edge; steps.
+    generalize dependent l1.
+    generalize dependent l2.
+    generalize dependent p1.
+    induction p2; intros.
+    + rewrite_anywhere app_nil_l.
+      simpl in *.
+      eapply reachable_path_is_reachable; destructs; eauto.
+      apply in_app_iff; steps.
+    + simpl in H.
+      destruct_match; [apply_anywhere app_eq_nil; steps |].
+      rewrite <- matched in *. destructs; eauto.
+  Qed.
+
+
+
+  Lemma reachable_path_assignment :
+    forall σ σ' C ω ω' p f l l',
+      (getObj σ l) = Some (C, ω) ->
+      ω' = [f ↦ l']ω ->
+      σ' = [l ↦ (C, ω')]σ ->
+      reachable_path σ' p ->
+      contains_edge p l l' \/ reachable_path σ p.
+  Proof.
+    intros.
+    pose proof (contains_edge_dec p l l') as [Hedge | Hedge]; eauto.
+    right.
+    induction p; eauto.
+    (* pose proof (PeanoNat.Nat.eq_dec a l') as [Ha | Ha]. *)
+    simpl in H2.
+    destruct_match; [steps ; unfold dom in *; rewrite_anywhere update_one3 => // |].
+    subst. destructs. intuition auto. simpl.
+    split.
+    + clear H2. clear H1. unfold reachable_one_step in *; steps.
+      destruct (PeanoNat.Nat.eq_dec l n); steps.
+      ++ rewrite_anywhere getObj_update1; eauto using getObj_dom.
+         invert_constructor_equalities; steps.
+         repeat eexists || eassumption. unfold getVal in *.
+         destruct (PeanoNat.Nat.eq_dec f f0); steps.
+         +++ rewrite_anywhere update_one1 ; eauto using nth_error_Some.
+             invert_constructor_equalities; steps.
+             exfalso; apply Hedge.
+             unfold contains_edge. exists l0, []; steps.
+             erewrite <- update_one3.
+             eapply nth_error_Some.
+             erewrite H0 => //.
+         +++ rewrite_anywhere update_one2; eauto .
+         +++ unfold dom in *. erewrite_anywhere update_one3; eauto.
+      ++ rewrite_anywhere getObj_update2; eauto using getObj_dom.
+         repeat eexists || eassumption.
+         unfold dom in *. erewrite <- update_one3; eauto.
+    + apply H2; clear H2.
+      unfold reachable_one_step, contains_edge in *.
+      intros. destructs.
+      apply Hedge. exists p1, (a::p2). rewrite H2.
+      rewrite app_comm_cons => //.
+  Qed.
+
+
 
 
 
