Scopability.v
@@ -185,18 +185,29 @@ Module Scopability.
     split.
     + (* σ1 ⇝ σ2' ⋖ L1 *)
       split. apply (proj1 H).
-      move => σ0 L L0 H_dom1 H_dom2' H_subL H_subL0 A1 A2.
+      move => σ0 L0 L H_dom1 H_dom2' H_subL H_subL0 A1 A2.
       assert (dom σ2 = dom σ2') as H_dom22'. rewrite /dom H4 update_one3 => //.
       move :(H_dom2') => H_dom2. rewrite -H_dom22' in H_dom2.
+      assert ((σ0, L0) ⋖ (σ2, L)) as B1 by (apply H; eauto).
+      assert ((σ0, L0) ⋖ (σ2, {l'})) as C1. {
+        eapply (scoping_transitivity _ σ1 _ L0 L1 {l'} ); eauto.
+        apply H.
+      }
       unfold scoping; simpl.
       intros. move: H8 => [l2 [Hl2 D1]].
-      apply (reachable_path_reachability σ2' l2 l0) in D1.
-      move: D1 => [p D1].
-      pose proof (in_dec EqNat.eq_nat_decide l
+      move: (proj2 (iff_and (reachable_path_reachability σ2' l2 l0)) D1) => [[D2 D3] | [p D2]].
+      ++ rewrite <- D2 in *. apply B1; simpl; eauto.
+         intros l3 Hl3. unfold dom in *. erewrite <- update_one3; steps; eauto.
+         eexists; split; eauto; try apply rch_heap. unfold dom in *. erewrite <- update_one3; steps; eauto.
+      ++ destruct (reachable_path_assignment _ _ _ _ _ _ _ _ _ H2 H3 H4 D2).
+         +++ pose proof (reachable_path_split_on_edge). admit.
+         +++ apply B1; simpl; eauto.
+             intros l3 Hl3. unfold dom in *. erewrite <- update_one3; steps; eauto.
+             exists l2 ; split => // .
+             apply reachable_path_reachability; right; eauto.
 
+    + admit.
 
-      intros _ _ l2 _ D1. simpl in D1. simpl.
-      admit. (* Reasonning on graphs *)
   Admitted.
 
   Definition codom (ρ: Env) : (LocSet):=
